\documentclass[12pt]{article}
\usepackage{a4wide, amsfonts, epsfig}
\newcommand\soln{\noindent\textit{Solution:} }

%NOTE that the year before has an extra inhomogeneous ode example
%
%

%skyline stuff
\font\upright=cmu10 scaled\magstep1
\setlength{\unitlength}{0.012500in}
\begingroup\makeatletter\ifx\SetFigFont\undefined
\def\x#1#2#3#4#5#6#7\relax{\def\x{#1#2#3#4#5#6}}%
\expandafter\x\fmtname xxxxxx\relax \def\y{splain}%
\ifx\x\y   % LaTeX or SliTeX?
\gdef\SetFigFont#1#2#3{%
  \ifnum #1<17\tiny\else \ifnum #1<20\small\else
  \ifnum #1<24\normalsize\else \ifnum #1<29\large\else
  \ifnum #1<34\Large\else \ifnum #1<41\LARGE\else
     \huge\fi\fi\fi\fi\fi\fi
  \csname #3\endcsname}%
\else
\gdef\SetFigFont#1#2#3{\begingroup
  \count@#1\relax \ifnum 25<\count@\count@25\fi
  \def\x{\endgroup\@setsize\SetFigFont{#2pt}}%
  \expandafter\x
    \csname \romannumeral\the\count@ pt\expandafter\endcsname
    \csname @\romannumeral\the\count@ pt\endcsname
  \csname #3\endcsname}%
\fi
\fi\endgroup

\begin{document}
\begin{center}
{\bf 2E2 Tutorial Sheet 14 Second Term}\footnote{Conor
Houghton, {\tt houghton@maths.tcd.ie} and {\tt
http://www.maths.tcd.ie/\char126 houghton/ 2E2.html}}
\\[1cm]
 10 February 2006
\end{center}
{
\noindent {\bf Useful facts:}\\
\begin{itemize}
\item The first order differential equation $y'=ry+f(t)$ has solution
\begin{equation}
y=Ce^{rt}+e^{rt}\int^t_0{f(\tau)e^{-r\tau}d\tau}
\end{equation}
\item To solve the inhomogeneous system ${\bf y}'=A{\bf y}+{\bf g}$ substitute 
\begin{equation}
{\bf y}=f_1{\bf x}_1+f_2{\bf x}_2
\end{equation}
where ${bf x}_1$ and ${\bf x}_2$ are the eigenvectors of $A$. You should also
split ${\bf g}$ up as ${\bf g}=h_1{\bf x}_1+h_2{\bf x}_2.$ This will
give you two independant first order inhomogeneous equations, one for
${\bf x}_1$ and one for ${\bf x}_2$.
\item Here is an example of converting the second order differential equation $y''+2y'+7y=0$ into a system first order differential equations. First rename $y_1=y$ and define $y_2=y_1'$, now, $y_2'=y_1''$ which we know from the original equation:
\begin{equation}
y_1''=y''=-2y'-7y
\end{equation}
but $y'$ is $y_2$ and $y$ is $y_1$, hence
\begin{eqnarray}
y_1'&=&y_2\cr
y_2'&=&-7y_1-2y_2
\end{eqnarray} 
\end{itemize}
\newpage
\noindent{\bf Questions}
\begin{enumerate}
\item (2) Find the solution to 
\begin{equation}
y'-2y=-t
\end{equation}
\vskip .5cm
\item (3) Find the general solution to
\begin{eqnarray}
y_1'&=&5y_2-23\nonumber\\ y_2'&=&5y_1+15.
\end{eqnarray}
with $y_1(0)=-3$ and $y_2(0)=5$.
\vskip .5cm
\item (2) Find the  general solution to
\begin{eqnarray}
y_1'&=&y_1+3y_2+e^t\nonumber\\
y_2'&=&3y_1+y_2
\end{eqnarray}
\vskip .5cm
\item (1) Rewrite $y''+4y'-3y=0$ as a system of two first order
differential equations.
\end{enumerate}
}
\end{document}



